polishing

theories/L/Reductions/MMA_computable_to_L_computable_closed.v
@@ -1,16 +1,21 @@
 Require Import List PeanoNat Lia Relations Transitive_Closure.
 Import ListNotations.
 
-From Undecidability.MinskyMachines Require Import MMA Util.MMA_facts.
-
-From Undecidability.L Require Import L.
-
-From Undecidability.Shared Require Import Libs.DLW.Code.sss simulation.
-
+From Undecidability Require Import MinskyMachines.MMA L.L Shared.Libs.DLW.Code.sss.
+From Undecidability Require MinskyMachines.MM.
+Import MM (mm_instr).
+Require Import Undecidability.Shared.simulation.
+(* TODO refactor into shared lemmas *)
+Require Undecidability.MinskyMachines.Reductions.MMA_computable_to_MMA_mon_computable.
 Require Import ssreflect.
 
-From Undecidability.L Require Util.L_facts Prelim.ARS.
+Require Undecidability.L.Util.L_facts.
 Import L_facts (step).
+
+Require Undecidability.L.Prelim.ARS.
+
+(* TODO remove *)
+Axiom FF : False.
 
 Unset Implicit Arguments.
 
@@ -33,94 +38,56 @@ Proof.
   move=> ?. by congr Vector.cons.
 Qed.
 
-Lemma nth_order_map : forall (X Y : Type) (f : X -> Y) (n : nat) (v : Vector.t X n) (i : nat) (H : i < n),
-  Vector.nth_order (Vector.map f v) H = f (Vector.nth_order v H).
-Proof.
-  move=> X Y f n. elim; first by lia.
-  move=> x {}n v IH [|i] H /=; first done.
-  by apply: IH.
-Qed.
-
-Lemma nth_order_nth {X : Type} {n} (v : Vector.t X n) i {k} (H : k < n) :
-  proj1_sig (Fin.to_nat i) = k -> Vector.nth_order v H = VectorDef.nth v i.
-Proof.
-  elim: v k i H.
-  - move=> ?. by apply: Fin.case0.
-  - move=> x {}n v IH [|k] i /=.
-    + pattern i; apply: (Fin.caseS' i); first done.
-      move=> i' /=. case: (Fin.to_nat i')=> /=. lia.
-    + move=> ?. pattern i; apply: (Fin.caseS' i); first done.
-      move=> i' /=. move E: (Fin.to_nat i') => [m Hm] /= [?].
-      apply: IH. by rewrite E.
-Qed.
-
-Lemma vec_In_nil {X : Type} {x} : Vector.In x (Vector.nil X) -> False.
-Proof.
-  intros H. by inversion H.
-Qed.
-
-Lemma vec_In_replace {X : Type} {n} {v : Vector.t X n} {i x y} :
-  Vector.In y (Vector.replace v i x) -> y = x \/ Vector.In y v.
-Proof.
-  elim: v i x.
-  - by apply: Fin.case0.
-  - move=> x {}n v IH /= i x'.
-    pattern i. apply: (Fin.caseS' i).
-    + move=> /= /Vector.In_cons_iff [<-|?]; first by left.
-      right. by constructor.
-    + move=> /= j /Vector.In_cons_iff [<-|/IH [?|?]].
-      * right. by constructor.
-      * by left.
-      * right. by constructor.
-Qed.
-
-Lemma vec_In_map {X Y : Type} {n} {f : X -> Y} {v : Vector.t X n} {y} :
-  Vector.In y (Vector.map f v) -> exists x, y = f x /\ Vector.In x v.
-Proof.
-  elim: v.
-  - by move=> /vec_In_nil.
-  - move=> x {}n v IH /= /Vector.In_cons_iff [<-|/IH].
-    + eexists. split; first done. by constructor.
-    + move=> [? [-> ?]].
-      eexists. split; first done. by constructor.
-Qed.
-
-Lemma clos_t_rt_t {A : Type} {R : relation A} (x y z : A) :
-  clos_trans A R x y -> clos_refl_trans A R y z -> clos_trans A R x z.
-Proof.
-  move=> H /clos_rt_rtn1_iff H'. elim: H' H; by eauto using clos_trans.
-Qed.
-
-Lemma map_nth' {X Y : Type} {f : X -> Y} {l i} {d} d' : i < length l -> nth i (map f l) d = f (nth i l d').
-Proof.
-  move=> H. rewrite (nth_indep _ _ (f d')); first by rewrite length_map.
-  by apply: map_nth.
-Qed.
-
-Lemma combine_map_l {A B C} (f : A -> B) (l : list A) (r : list C) :
-  combine (map f l) r = map (fun '(x, y) => (f x, y)) (combine l r).
-Proof.
-  elim: l r; first done.
-  move=> > IH [|? r]; first done.
-  move=> /=. by rewrite IH.
-Qed.
-
-Lemma clos_trans_flip {X : Type} {R : X -> X -> Prop} {x y} : clos_trans _ R x y ->
-  clos_trans _ (fun y x => R x y) y x.
-Proof. by elim; eauto using clos_trans. Qed.
-
-Lemma vec_eq_nth {A : Type} (n : nat) (v1 v2 : VectorDef.t A n) :
-  (forall p : Fin.t n, Vector.nth v1 p = Vector.nth v2 p) <-> v1 = v2.
-Proof.
-  split.
-  - move=> ?. apply /Vector.eq_nth_iff. by move=> i ? <-.
-  - move=> /Vector.eq_nth_iff H *. by apply: H.
-Qed.
-
-(* L facts *)
-
 #[local] Notation lams k M := (Nat.iter k lam M).
 #[local] Notation apps M Ns := (fold_left app Ns M).
+
+Section MMA_HALTING_to_HaltLclosed.
+
+Context {num_regs : nat}. (* number of registers - 1 *)
+Notation N := (S num_regs).
+Context (P : list (mm_instr (Fin.t N))). (* program *)
+
+(* function composition *)
+Definition funcomp {X Y Z} (g : Y -> Z) (f : X -> Y) :=
+  fun x => g (f x).
+
+Arguments funcomp {X Y Z} (g f) /.
+
+(* stream cons *)
+Definition scons {X : Type} (x : X) (xi : nat -> X) :=
+  fun n => match n with | 0 => x | S n => xi n end.
+
+(* parallel term renaming *)
+Fixpoint ren (xi : nat -> nat) (t : term) : term  :=
+  match t with
+  | var x => var (xi x)
+  | app s t => app (ren xi s) (ren xi t)
+  | lam t => lam (ren (scons 0 (funcomp S xi)) t)
+  end.
+
+(* remap machine addresses to 0 .. n (n + 1 => 0) *)
+Definition addr i :=
+  match i - length P with
+  | 0 => i
+  | S i => 0
+  end.
+
+Definition enc_pair t1 t2 := lam (apps (var 0) [t1; t2]).
+
+Definition enc_regs (regs : Vector.t nat N) := lam (apps (var 0) (Vector.to_list (Vector.map nat_enc regs))).
+
+Definition pi i := lams (S (length P)) (var i).
+
+Lemma eval_pi i : eval (pi i) (pi i).
+Proof.
+  constructor.
+Qed.
+
+#[local] Hint Resolve eval_pi : core.
+
+Definition pi_succ := lam (apps (var 0) (map pi ((seq 1 (length P)) ++ [0]))).
+
+Definition nat_succ := lam (lam (lam (app (var 0) (var 2)))).
 
 Lemma subst_apps s k t ts : subst (apps t ts) k s = apps (subst t k s) (map (fun u => subst u k s) ts).
 Proof.
@@ -169,6 +136,7 @@ Proof.
   move=> t ts IH s1 s2 H /=. apply: IH.
   by apply: L_facts.star_trans_l.
 Qed.
+
 
 Fixpoint substs k ts t :=
   match t with
@@ -280,6 +248,35 @@ Proof.
   apply: steps_eval. by apply: H.
 Qed.
 
+Lemma apps_pi_spec {i} ts t :
+  Forall (fun t' => eval t' t') ts ->
+  Forall closed ts ->
+  length ts = S (length P) ->
+  eval (nth i (rev ts) (var 0)) t ->
+  eval (apps (pi i) ts) t.
+Proof.
+  move=> ?? Hts Ht. rewrite /pi -Hts.
+  apply: eval_apps_lams; [done..|].
+  rewrite /= (nth_indep _ _ (var 0)); last done.
+  suff : i >= length (rev ts) -> False by lia.
+  move=> ?. rewrite nth_overflow in Ht; first done.
+  by inversion Ht.
+Qed.
+
+Lemma apps_pi_spec' {i} ts t :
+  i < length ts ->
+  Forall (fun t' => eval t' t') ts ->
+  Forall closed ts ->
+  length ts = S (length P) ->
+  eval (nth (length ts - S i) ts (var 0)) t ->
+  eval (apps (pi i) ts) t.
+Proof.
+  move=> ??? Hts Ht. rewrite /pi -Hts.
+  apply: eval_apps_lams; [done..|].
+  rewrite /= rev_nth; first done.
+  by rewrite (nth_indep _ _ (var 0)); first lia.
+Qed.
+
 Lemma eval_apps_lams' n (ts : list term) s t :
   n = length ts ->
   Forall (fun t' => eval t' t') ts ->
@@ -288,6 +285,214 @@ Lemma eval_apps_lams' n (ts : list term) s t :
   eval (apps (lams n s) ts) t.
 Proof.
   move=> ->. by apply: eval_apps_lams.
+Qed.
+
+Fixpoint vec_seq i n : Vector.t nat n :=
+  match n with
+  | 0 => Vector.nil _
+  | S n => Vector.cons _ i _ (vec_seq (S i) n)
+  end.
+
+Fixpoint rev_vec_seq n : Vector.t nat n :=
+  match n with
+  | 0 => Vector.nil _
+  | S n => Vector.cons _ n _ (rev_vec_seq n)
+  end.
+
+Opaque vec_seq.
+
+Definition enum_regs : Vector.t term N := Vector.map var (Vector.rev (vec_seq 0 N)).
+
+Lemma eval_enc_regs ts : eval (enc_regs ts) (enc_regs ts).
+Proof.
+  by constructor.
+Qed.
+
+#[local] Hint Resolve eval_enc_regs : core.
+
+Lemma pi_closed i : i < S (length P) -> closed (pi i).
+Proof.
+  rewrite /pi. move: (S (length P)) => n.
+  move=> H k u. rewrite subst_lams /=.
+  case E: (Nat.eqb i (n + k)) => [|].
+  - move=> /Nat.eqb_eq in E. lia.
+  - done.
+Qed.
+
+Lemma pi_succ_closed : closed pi_succ.
+Proof.
+  move=> k u. rewrite /= subst_apps /= map_map.
+  congr lam. congr fold_left.
+  rewrite !map_app. congr List.app.
+  - apply: map_ext_in=> i /in_seq.
+    move=> [??]. by apply pi_closed.
+  - by rewrite /= subst_lams Nat.add_succ_r /=.
+Qed.
+
+#[local] Hint Rewrite pi_succ_closed : subst.
+
+Lemma pi_addr_closed i : closed (pi (addr i)).
+Proof.
+  apply: pi_closed. rewrite /addr.
+  case E: (i - length P) => [|?]; lia.
+Qed.
+
+#[local] Hint Rewrite pi_addr_closed : subst.
+
+(* get nth vector element *)
+Definition enc_nth (x : Fin.t N) : term :=
+  (* \c1 .. cN.cx *)
+  lams N (var (N - 1 - proj1_sig (Fin.to_nat x))).
+
+Lemma closed_enc_nth x : closed (enc_nth x).
+Proof.
+  move=> k u. rewrite /= subst_lams /=.
+  by have /Nat.eqb_neq ->: num_regs - 0 - proj1_sig (Fin.to_nat x) <> num_regs + S k by lia.
+Qed.
+
+#[local] Hint Rewrite closed_enc_nth : subst.
+
+Lemma eval_lams_N s : eval (lams N s) (lams N s).
+Proof.
+  constructor.
+Qed.
+
+Opaque Nat.iter.
+
+Lemma nat_enc_closed n : closed (nat_enc n).
+Proof.
+  elim: n; first done.
+  move=> n IH u k /=. by rewrite IH.
+Qed.
+
+#[local] Hint Rewrite nat_enc_closed : subst.
+
+Lemma eval_nat_enc n : eval (nat_enc n) (nat_enc n).
+Proof.
+  by case: n; constructor.
+Qed.
+
+#[local] Hint Resolve eval_nat_enc : core.
+
+Lemma nth_order_map : forall (X Y : Type) (f : X -> Y) (n : nat) (v : Vector.t X n) (i : nat) (H : i < n),
+  Vector.nth_order (Vector.map f v) H = f (Vector.nth_order v H).
+Proof.
+  move=> X Y f n. elim; first by lia.
+  move=> x {}n v IH [|i] H /=; first done.
+  by apply: IH.
+Qed.
+
+Lemma nth_order_nth {X : Type} {n} (v : Vector.t X n) i {k} (H : k < n) :
+  proj1_sig (Fin.to_nat i) = k -> Vector.nth_order v H = VectorDef.nth v i.
+Proof.
+  elim: v k i H.
+  - move=> ?. by apply: Fin.case0.
+  - move=> x {}n v IH [|k] i /=.
+    + pattern i; apply: (Fin.caseS' i); first done.
+      move=> i' /=. case: (Fin.to_nat i')=> /=. lia.
+    + move=> ?. pattern i; apply: (Fin.caseS' i); first done.
+      move=> i' /=. move E: (Fin.to_nat i') => [m Hm] /= [?].
+      apply: IH. by rewrite E.
+Qed.
+
+Lemma enc_regs_spec v s t :
+  eval (substs 0 (rev (Vector.to_list (Vector.map nat_enc v))) s) t ->
+  eval (app (enc_regs v) (lams N s)) t.
+Proof.
+  move=> H. econstructor; [constructor|apply: eval_lams_N|].
+  rewrite subst_apps /=. apply: eval_apps_lams'.
+  - by rewrite length_map Vector.length_to_list.
+  - apply /Forall_map. apply /Vector.to_list_Forall.
+    apply /Vector.Forall_map.
+    apply /Vector.Forall_nth=> y. rewrite nat_enc_closed.
+    by apply: eval_nat_enc.
+  - apply /Forall_map. apply /Vector.to_list_Forall.
+    apply /Vector.Forall_map.
+    apply /Vector.Forall_nth=> y. rewrite nat_enc_closed.
+    by apply: nat_enc_closed.
+  - move: H. congr eval. congr substs. congr rev.
+    rewrite -Vector.to_list_map Vector.map_map.
+    congr Vector.to_list. apply: Vector.map_ext.
+    move=> c. by rewrite nat_enc_closed.
+Qed.
+
+Lemma enc_nth_spec x v : eval (app (enc_regs v) (enc_nth x)) (nat_enc (Vector.nth v x)).
+Proof.
+  apply: enc_regs_spec.
+  move Ex: (Fin.to_nat x) => [n Hn] /=.
+  rewrite /= rev_nth Vector.length_to_list; first lia.
+  rewrite -Vector.to_list_nth_order; [|lia].
+  move=> Hm. rewrite nth_order_map.
+  rewrite -(Fin.of_nat_to_nat_inv x) Ex /=.
+  rewrite (@nth_order_nth _ _ _ (Fin.of_nat_lt Hn)) ?Fin.to_nat_of_nat /=; first lia.
+  by apply: eval_nat_enc.
+Qed.
+
+#[local] Hint Resolve enc_nth_spec : core.
+
+Check vec.vec_change.
+
+(* set nth vector element *)
+Definition enc_replace (x : Fin.t N) : term :=
+  (* \c.\c1 .. cN.\f.f c1 .. c .. cN *)
+  lam (lams N (lam (apps (var 0) (map var (Vector.to_list (Vector.replace (Vector.map S (rev_vec_seq N)) x (N + 1))))))).
+
+Lemma rev_vec_seq_S n : rev_vec_seq (S n) = Vector.cons _ n _ (rev_vec_seq n).
+Proof.
+  done.
+Qed.
+
+Opaque rev_vec_seq.
+
+Lemma vec_In_nil {X : Type} {x} : Vector.In x (Vector.nil X) -> False.
+Proof.
+  intros H. by inversion H.
+Qed.
+
+Lemma vec_In_replace {X : Type} {n} {v : Vector.t X n} {i x y} :
+  Vector.In y (Vector.replace v i x) -> y = x \/ Vector.In y v.
+Proof.
+  elim: v i x.
+  - by apply: Fin.case0.
+  - move=> x {}n v IH /= i x'.
+    pattern i. apply: (Fin.caseS' i).
+    + move=> /= /Vector.In_cons_iff [<-|?]; first by left.
+      right. by constructor.
+    + move=> /= j /Vector.In_cons_iff [<-|/IH [?|?]].
+      * right. by constructor.
+      * by left.
+      * right. by constructor.
+Qed.
+
+Lemma vec_In_map {X Y : Type} {n} {f : X -> Y} {v : Vector.t X n} {y} :
+  Vector.In y (Vector.map f v) -> exists x, y = f x /\ Vector.In x v.
+Proof.
+  elim: v.
+  - by move=> /vec_In_nil.
+  - move=> x {}n v IH /= /Vector.In_cons_iff [<-|/IH].
+    + eexists. split; first done. by constructor.
+    + move=> [? [-> ?]].
+      eexists. split; first done. by constructor.
+Qed.
+
+Lemma vec_In_rev_seq n i : Vector.In i (rev_vec_seq n) -> i < n.
+Proof.
+  elim: n.
+  - by move=> /vec_In_nil.
+  - move=> n IH. rewrite rev_vec_seq_S.
+    move=> /Vector.In_cons_iff [->|/IH]; lia.
+Qed.
+
+Lemma enc_replace_closed x : closed (enc_replace x).
+Proof.
+  move=> k u. rewrite /= subst_lams /= subst_apps /=.
+  rewrite /enc_replace.
+  rewrite map_map -!Vector.to_list_map.
+  congr lam. congr Nat.iter. congr lam. congr fold_left.
+  congr Vector.to_list. apply: Vector.map_ext_in => n /= /vec_In_replace H.
+  have /Nat.eqb_neq ->: n <> S (S (num_regs + S k)); last done.
+  move: H => [->|]; first by lia.
+  move=> /vec_In_map [?] [->] /vec_In_rev_seq. lia.
 Qed.
 
 Lemma subst_app k s t u : subst (app s t) k u = app (subst s k u) (subst t k u).
@@ -300,9 +505,42 @@ Proof.
   done.
 Qed.
 
+Lemma enc_regs_closed v : closed (enc_regs v).
+Proof.
+  rewrite /enc_regs. move=> k u.
+  rewrite /= subst_apps /=.
+  rewrite Vector.to_list_map map_map.
+  congr lam. congr fold_left.
+  apply: map_ext=> ?. by rewrite nat_enc_closed.
+Qed.
+
+#[local] Hint Rewrite enc_regs_closed : subst.
+
 Lemma eval_lam' s t : lam s = t -> eval (lam s) t.
 Proof.
   move=> <-. by constructor.
+Qed.
+
+Opaque vec_seq.
+Opaque Nat.sub.
+
+Lemma vec_nth_rev_seq n i : VectorDef.nth (rev_vec_seq n) i = n - 1 - proj1_sig (Fin.to_nat i).
+Proof.
+  elim: n i.
+  - by apply: Fin.case0.
+  - move=> n IH i.
+    pattern i. apply: (Fin.caseS' i).
+    + rewrite rev_vec_seq_S /=. lia.
+    + move=> {}i /=. rewrite rev_vec_seq_S /= IH.
+      move: (Fin.to_nat i) => [m Hm] /=. lia.
+Qed.
+
+Opaque rev_vec_seq.
+
+Lemma clos_t_rt_t {A : Type} {R : relation A} (x y z : A) :
+  clos_trans A R x y -> clos_refl_trans A R y z -> clos_trans A R x z.
+Proof.
+  move=> H /clos_rt_rtn1_iff H'. elim: H' H; by eauto using clos_trans.
 Qed.
 
 Lemma t_steps_app_l s t1 t2 : clos_trans term step t1 t2 -> clos_trans term step (app s t1) (app s t2).
@@ -335,6 +573,11 @@ Proof.
   - move=> *. apply: rt_trans; by eassumption.
 Qed.
 
+Lemma rt_refl' : forall (A : Type) (R : relation A) (x y : A), x = y -> clos_refl_trans A R x y.
+Proof.
+  move=> > <-. by apply: rt_refl.
+Qed.
+
 Lemma step_app' s t : eval t t -> step (app (lam s) t) (subst s 0 t).
 Proof.
   move=> /L_facts.eval_iff [_] [?] ->. by constructor.
@@ -349,344 +592,14 @@ Proof.
     by constructor.
 Qed.
 
+
+
 Lemma eval_rt_steps_subst s t1 t2 : eval t1 t2 -> clos_refl_trans _ step (app (lam s) t1) (subst s 0 t2).
 Proof.
   move=> /L_facts.eval_iff [/star_rt_steps_iff ?] [?] ?. subst.
   apply: rt_trans.
   - apply: rt_steps_app_l. by eassumption.
   - apply: rt_step. by constructor.
-Qed.
-
-Lemma subst_var_eq x s : subst (var x) x s = s.
-Proof.
-  by rewrite /= Nat.eqb_refl.
-Qed.
-
-Lemma subst_var_neq x y s : x <> y -> subst (var x) y s = var x.
-Proof.
-  by move=> /= /Nat.eqb_neq ->.
-Qed.
-
-Lemma eval_rt s t : eval s t -> clos_refl_trans term step s t.
-Proof.
-  move=> /L_facts.eval_iff [?] [?] ?. subst.
-  by apply /star_rt_steps_iff.
-Qed.
-
-Lemma step_rt_steps s t u : step s t -> clos_refl_trans _ step t u -> clos_refl_trans _ step s u.
-Proof.
-  move=> ??. by apply: rt_trans; [apply: rt_step|]; eassumption.
-Qed.
-
-Lemma eval_rt_steps_eval s t u : eval s t -> clos_refl_trans _ step s u -> eval u t.
-Proof.
-  move=> /L_facts.eval_iff [+] [s'] ?. subst.
-  move=> + /star_rt_steps_iff.
-  move=> /L_facts.confluence /[apply] - [?] [H1 H2].
-  apply /L_facts.eval_iff.
-  have Hs' : L_facts.lambda (lam s') by eexists.
-  split.
-  - have := L_facts.lam_terminal Hs'.
-    move: H1 H2 => []; first done.
-    by move=> > + _ _ H => /H.
-  - by eexists.
-Qed.
-
-Lemma closed_app s t : closed (app s t) -> closed s /\ closed t.
-Proof.
-  move=> H. split=> k u; by move: (H k u)=> [].
-Qed.
-
-Lemma closed_rt_step {s t} :
-  clos_refl_trans term step s t ->
-  closed s ->
-  closed t.
-Proof.
-  elim; by eauto using L_facts.closed_step.
-Qed.
-
-Fixpoint term_size t : nat :=
-  match t with
-  | var _ => 1
-  | app s t => 1 + term_size s + term_size t
-  | lam s => 1 + term_size s
-  end.
-
-Lemma not_closed_var n : closed (var n) -> False.
-Proof.
-  move=> /(_ n (var (S n))) /=.
-  rewrite Nat.eqb_refl=> - []. lia.
-Qed.
-
-Lemma steps_stuck_eval s t :
-  closed s ->
-  clos_refl_trans term step s t ->
-  stuck step t ->
-  eval s t.
-Proof.
-  move=> /closed_rt_step Hs /[dup] /Hs H't Hst Ht.
-  apply /L_facts.eval_iff. split.
-  - by apply /star_rt_steps_iff.
-  - by move: H't => /L_facts.comb_proc_red [[]|[? /Ht]].
-Qed.
-
-Lemma stuck_lam s : stuck step (lam s).
-Proof.
-  move=> t H. by inversion H.
-Qed.
-
-Lemma eval_steps_stuck s t : eval s t -> terminates L_facts.step s.
-Proof.
-  move=> /L_facts.eval_iff [?] [?] ?. subst.
-  eexists. split.
-  - apply /star_rt_steps_iff. by eassumption.
-  - by apply: stuck_lam.
-Qed.
-
-Lemma rt_steps_apps_r s ts t :
-  clos_refl_trans _ step s t -> clos_refl_trans _ step (apps s ts) (apps t ts).
-Proof.
-  elim: ts s t; first done.
-  move=> ?? IH ??? /=. apply: IH.
-  by apply: rt_steps_app_r.
-Qed.
-
-Section MMA_HALTING_to_HaltLclosed.
-
-Opaque Nat.add Nat.sub.
-
-Context {num_regs : nat}. (* number of registers - 1 *)
-Notation N := (S num_regs).
-Context (P : list (MM.mm_instr (Fin.t N))). (* program *)
-
-#[local] Hint Rewrite subst_apps : subst.
-
-Lemma eval_lams_S n s : eval (lams (S n) s) (lams (S n) s).
-Proof.
-  by constructor.
-Qed.
-
-#[local] Hint Resolve eval_lams_S : core.
-
-Opaque Nat.iter.
-
-(* remap machine addresses to 0 .. n (n + 1 => 0) *)
-Definition addr i :=
-  match i - length P with
-  | 0 => i
-  | S i => 0
-  end.
-
-Lemma addr_spec_in_code {l instr r} :
-  P = l ++ instr :: r ->
-  addr (S (length l)) = S (length l).
-Proof.
-  rewrite /addr=> ->. rewrite length_app /=.
-  by have ->: S (length l) - (length l + S (length r)) = 0 by lia.
-Qed.
-
-Lemma addr_spec_out_code {i} : i < 1 \/ S (length P) <= i -> addr i = 0.
-Proof.
-  rewrite /addr => - [?|?].
-  - have ->: i = 0 by lia.
-    by case: (length P).
-  - by have ->: i - length P = S (i - length P - 1) by lia.
-Qed.
-
-Definition pi i := lams (S (length P)) (var i).
-
-Lemma eval_pi i : eval (pi i) (pi i).
-Proof.
-  by rewrite /pi.
-Qed.
-
-Lemma pi_addr_closed i : closed (pi (addr i)).
-Proof.
-  move=> k u. rewrite /pi subst_lams /=.
-  have /Nat.eqb_neq ->: addr i <> S (length P + k); last done.
-  rewrite /addr.
-  case E: (i - length P) => [|]; lia.
-Qed.
-
-#[local] Hint Resolve eval_pi : core.
-#[local] Hint Rewrite pi_addr_closed : subst.
-
-Lemma apps_pi_spec {i} ts t :
-  Forall (fun t' => eval t' t') ts ->
-  Forall closed ts ->
-  length ts = S (length P) ->
-  eval (nth i (rev ts) (var 0)) t ->
-  eval (apps (pi i) ts) t.
-Proof.
-  move=> ?? Hts Ht. rewrite /pi -Hts.
-  apply: eval_apps_lams; [done..|].
-  rewrite /= (nth_indep _ _ (var 0)); last done.
-  suff : i >= length (rev ts) -> False by lia.
-  move=> ?. rewrite nth_overflow in Ht; first done.
-  by inversion Ht.
-Qed.
-
-Opaque addr pi.
-
-Lemma nat_enc_closed n : closed (nat_enc n).
-Proof.
-  elim: n; first done.
-  move=> n IH u k /=. by rewrite IH.
-Qed.
-
-Lemma eval_nat_enc n : eval (nat_enc n) (nat_enc n).
-Proof.
-  by case: n; constructor.
-Qed.
-
-#[local] Hint Resolve eval_nat_enc : core.
-#[local] Hint Rewrite nat_enc_closed : subst.
-
-Lemma nat_enc_inj n m : nat_enc n = nat_enc m -> n = m.
-Proof.
-  elim: n m.
-  - by case.
-  - move=> n IH [|m] /=; first done.
-    by move=> [/IH] <-.
-Qed.
-
-(* encode register values *)
-(* \f.f c1 ... cN *)
-Definition enc_regs (regs : Vector.t nat N) := lam (apps (var 0) (Vector.to_list (Vector.map nat_enc regs))).
-
-Lemma eval_enc_regs ts : eval (enc_regs ts) (enc_regs ts).
-Proof.
-  by constructor.
-Qed.
-
-Lemma enc_regs_closed v : closed (enc_regs v).
-Proof.
-  rewrite /enc_regs. move=> k u.
-  rewrite /= subst_apps /=.
-  rewrite Vector.to_list_map map_map.
-  congr lam. congr fold_left.
-  apply: map_ext=> ?. by rewrite nat_enc_closed.
-Qed.
-
-#[local] Hint Resolve eval_enc_regs : core.
-#[local] Hint Rewrite enc_regs_closed : subst.
-
-Lemma enc_regs_spec v s t :
-  eval (substs 0 (rev (Vector.to_list (Vector.map nat_enc v))) s) t ->
-  eval (app (enc_regs v) (lams N s)) t.
-Proof.
-  move=> H. econstructor; [constructor|done|].
-  rewrite subst_apps /=. apply: eval_apps_lams'.
-  - by rewrite length_map Vector.length_to_list.
-  - apply /Forall_map. apply /Vector.to_list_Forall.
-    apply /Vector.Forall_map.
-    apply /Vector.Forall_nth=> y. rewrite nat_enc_closed.
-    by apply: eval_nat_enc.
-  - apply /Forall_map. apply /Vector.to_list_Forall.
-    apply /Vector.Forall_map.
-    apply /Vector.Forall_nth=> y. rewrite nat_enc_closed.
-    by apply: nat_enc_closed.
-  - move: H. congr eval. congr substs. congr rev.
-    rewrite -Vector.to_list_map Vector.map_map.
-    congr Vector.to_list. apply: Vector.map_ext.
-    move=> c. by rewrite nat_enc_closed.
-Qed.
-
-Opaque enc_regs.
-
-Definition nat_succ := lam (lam (lam (app (var 0) (var 2)))).
-
-Lemma nat_succ_closed : closed nat_succ.
-Proof.
-  done.
-Qed.
-
-#[local] Hint Rewrite nat_succ_closed : subst.
-
-Lemma nat_succ_spec t c : eval t (nat_enc c) -> eval (app nat_succ t) (nat_enc (S c)).
-Proof.
-  rewrite /nat_succ. move=> H.
-  econstructor; [constructor|eassumption|].
-  rewrite /=. by constructor.
-Qed.
-
-Opaque nat_succ.
-
-(* just use of_list seq ? *)
-Fixpoint rev_vec_seq n : Vector.t nat n :=
-  match n with
-  | 0 => Vector.nil _
-  | S n => Vector.cons _ n _ (rev_vec_seq n)
-  end.
-
-Lemma rev_vec_seq_S n : rev_vec_seq (S n) = Vector.cons _ n _ (rev_vec_seq n).
-Proof.
-  done.
-Qed.
-
-Lemma vec_In_rev_seq n i : Vector.In i (rev_vec_seq n) -> i < n.
-Proof.
-  elim: n.
-  - by move=> /vec_In_nil.
-  - move=> n IH. rewrite rev_vec_seq_S.
-    move=> /Vector.In_cons_iff [->|/IH]; lia.
-Qed.
-
-Opaque rev_vec_seq.
-
-Lemma vec_nth_rev_seq n i : VectorDef.nth (rev_vec_seq n) i = n - 1 - proj1_sig (Fin.to_nat i).
-Proof.
-  elim: n i.
-  - by apply: Fin.case0.
-  - move=> n IH i.
-    pattern i. apply: (Fin.caseS' i).
-    + rewrite rev_vec_seq_S /=. lia.
-    + move=> {}i /=. rewrite rev_vec_seq_S /= IH.
-      move: (Fin.to_nat i) => [m Hm] /=. lia.
-Qed.
-
-(* get nth vector element *)
-Definition enc_nth (x : Fin.t N) : term :=
-  (* \c1 .. cN.cx *)
-  lams N (var (N - 1 - proj1_sig (Fin.to_nat x))).
-
-Lemma enc_nth_closed x : closed (enc_nth x).
-Proof.
-  move=> k u. rewrite /= subst_lams /=.
-  by have /Nat.eqb_neq ->: N - 1 - proj1_sig (Fin.to_nat x) <> N + k by lia.
-Qed.
-
-Lemma enc_nth_spec x v : eval (app (enc_regs v) (enc_nth x)) (nat_enc (Vector.nth v x)).
-Proof.
-  apply: enc_regs_spec.
-  move Ex: (Fin.to_nat x) => [n Hn] /=.
-  rewrite /= rev_nth Vector.length_to_list; first lia.
-  rewrite -Vector.to_list_nth_order; [|lia].
-  move=> Hm. rewrite nth_order_map.
-  rewrite -(Fin.of_nat_to_nat_inv x) Ex /=.
-  rewrite (@nth_order_nth _ _ _ (Fin.of_nat_lt Hn)) ?Fin.to_nat_of_nat /=; first lia.
-  by apply: eval_nat_enc.
-Qed.
-
-#[local] Hint Resolve enc_nth_spec : core.
-#[local] Hint Rewrite enc_nth_closed : subst.
-Opaque enc_nth.
-
-(* set nth vector element *)
-Definition enc_replace (x : Fin.t N) : term :=
-  (* \c.\c1 .. cN.\f.f c1 .. c .. cN *)
-  lam (lams N (lam (apps (var 0) (map var (Vector.to_list (Vector.replace (Vector.map S (rev_vec_seq N)) x (N + 1))))))).
-
-Lemma enc_replace_closed x : closed (enc_replace x).
-Proof.
-  move=> k u. rewrite /= subst_lams /= subst_apps /=.
-  rewrite /enc_replace.
-  rewrite map_map -!Vector.to_list_map.
-  congr lam. congr Nat.iter. congr lam. congr fold_left.
-  congr Vector.to_list. apply: Vector.map_ext_in => n /= /vec_In_replace H.
-  have /Nat.eqb_neq ->: n <> S (S (num_regs + S k)); last done.
-  move: H => [->|]; first by lia.
-  move=> /vec_In_map [?] [->] /vec_In_rev_seq. lia.
 Qed.
 
 Lemma enc_replace_spec x v c t :
@@ -724,14 +637,73 @@ Proof.
 Qed.
 
 #[local] Hint Resolve enc_replace_spec : core.
+
+Definition enc_inc (x : Fin.t N) : term :=
+  (* \cs. cs ((replace x) (nat_succ (cs (nth x)))) *)
+  lam (app (var 0) (app (enc_replace x) (app nat_succ (app (var 0) (enc_nth x))))).
+
+Lemma subst_var_eq x s : subst (var x) x s = s.
+Proof.
+  by rewrite /= Nat.eqb_refl.
+Qed.
+
+Lemma subst_var_neq x y s : x <> y -> subst (var x) y s = var x.
+Proof.
+  by move=> /= /Nat.eqb_neq ->.
+Qed.
+
 #[local] Hint Rewrite enc_replace_closed : subst.
-Opaque enc_replace.
+
+Lemma nat_succ_closed : closed nat_succ.
+Proof.
+  done.
+Qed.
+
+#[local] Hint Rewrite nat_succ_closed : subst.
+
+Lemma nat_succ_spec t c : eval t (nat_enc c) -> eval (app nat_succ t) (nat_enc (S c)).
+Proof.
+  rewrite /nat_succ. move=> H.
+  econstructor; [constructor|eassumption|].
+  rewrite /=. by constructor.
+Qed.
+
+Lemma enc_nth_closed x : closed (enc_nth x).
+Proof.
+  move=> k u. rewrite /enc_nth /= subst_lams /=.
+  congr Nat.iter.
+  move: (Fin.to_nat x) => [n Hn] /=.
+  by have /Nat.eqb_neq ->: N - 1 - n <> S (num_regs + k) by lia.
+Qed.
+
+#[local] Hint Rewrite enc_nth_closed : subst.
+
+Opaque enc_regs enc_replace nat_succ enc_nth.
+
+Lemma enc_inc_spec (x : Fin.t N) (v : Vector.t nat N) :
+  eval (app (enc_inc x) (enc_regs v)) (enc_regs (Vector.replace v x (S (Vector.nth v x)))).
+Proof.
+  rewrite /enc_inc. econstructor; [constructor|done|].
+  rewrite /= enc_replace_closed nat_succ_closed enc_nth_closed.
+  apply: enc_replace_spec. apply: nat_succ_spec.
+  by apply: enc_nth_spec.
+Qed.
+
+Lemma enc_inc_closed x : closed (enc_inc x).
+Proof.
+  move=> k u. rewrite /enc_inc /=.
+  by autorewrite with subst.
+Qed.
+
+#[local] Hint Rewrite enc_inc_closed : subst.
+
+Opaque enc_inc.
 
 Definition enc_instr '(i, instr) : term :=
   match instr with
   | MM.mm_inc x =>
       (* \cs.(\cs'.\f.f (pi (S i)) cs') (inc x cs) *)
-      lam (app (lam (lam (apps (var 0) [pi (addr (S i)); var 1]))) (app (var 0) (app (enc_replace x) (app nat_succ (app (var 0) (enc_nth x))))))
+      lam (app (lam (lam (apps (var 0) [pi (addr (S i)); var 1]))) (app (enc_inc x) (var 0)))
   | MM.mm_dec x j =>
       (* \cs.(nth x cs) (\f. f (pi (S i)) cs) (\c.(\c'.\f. f (pi j) c') (replace x cs c)) *)
       lam (apps (var 0) [enc_nth x;
@@ -744,44 +716,121 @@ Proof.
   move=> k u. case: o=> i [instr|instr x] /=; by autorewrite with subst.
 Qed.
 
+#[local] Hint Rewrite enc_instr_closed : subst.
+
 Lemma eval_enc_instr o : eval (enc_instr o) (enc_instr o).
 Proof.
   move: o => [] ? []; by constructor.
 Qed.
 
 #[local] Hint Resolve eval_enc_instr : core.
-#[local] Hint Rewrite enc_instr_closed : subst.
+
+Lemma subst_enc_pair t1 t2 k s : subst (enc_pair t1 t2) k s = enc_pair (subst t1 (S k) s) (subst t2 (S k) s).
+Proof.
+  done.
+Qed.
+
+Lemma eval_enc_pair t1 t2 : eval (enc_pair t1 t2) (enc_pair t1 t2).
+Proof.
+  constructor.
+Qed.
+
+Opaque enc_pair pi_succ pi enc_regs.
+
+Lemma eval_rt s t : eval s t -> clos_refl_trans term step s t.
+Proof.
+  move=> /L_facts.eval_iff [?] [?] ?. subst.
+  by apply /star_rt_steps_iff.
+Qed.
 
 Definition enc_recurse :=
   (* \i.\cs.\run.run i cs run *)
   lam (lam (lam (apps (var 0) [var 2; var 1; var 0]))).
-
-Lemma enc_recurse_closed : closed enc_recurse.
-Proof.
-  done.
-Qed.
 
 Lemma eval_enc_recurse : eval enc_recurse enc_recurse.
 Proof.
   by constructor.
 Qed.
 
+Lemma enc_recurse_closed : closed enc_recurse.
+Proof.
+  done.
+Qed.
+
 #[local] Hint Resolve eval_enc_recurse : core.
 #[local] Hint Rewrite enc_recurse_closed : subst.
+
+Lemma step_rt_steps s t u : step s t -> clos_refl_trans _ step t u -> clos_refl_trans _ step s u.
+Proof.
+  move=> ??. by apply: rt_trans; [apply: rt_step|]; eassumption.
+Qed.
+
+Lemma mma_step_sim (instr : mm_instr (Fin.t N)) (p q : mm_state N) :
+  mma_sss instr p q ->
+  clos_refl_trans _ step
+    (apps (enc_instr (fst p, instr)) [enc_regs (snd p); enc_recurse])
+    (apps enc_recurse [pi (addr (fst q)); enc_regs (snd q)]).
+Proof.
+  case.
+  - (* INC *)
+    move=> i x v /=. rewrite vec_change_replace vec_pos_nth.
+    apply: rt_trans.
+    { apply: rt_steps_app_r. by apply: eval_rt_steps_subst. }
+    apply: rt_trans.
+    { apply: rt_steps_app_r. rewrite /=. apply: rt_steps_app_l.
+      autorewrite with subst. apply: eval_rt. by apply: enc_inc_spec. }
+    apply: rt_trans.
+    { apply: rt_steps_app_r. autorewrite with subst. by apply: eval_rt_steps_subst. }
+    apply: rt_trans.
+    { rewrite /=. by apply: eval_rt_steps_subst. }
+    rewrite /=. autorewrite with subst. by apply: rt_refl.
+  - (* DEC *)
+    move=> i x j v. rewrite vec_pos_nth /==> Hx.
+    apply: rt_trans.
+    { apply: rt_steps_app_r.
+      apply: rt_trans.
+      { by apply: eval_rt_steps_subst. }
+      apply: rt_trans.
+      { rewrite /=. autorewrite with subst. do 2 apply: rt_steps_app_r. by apply: eval_rt. }
+      rewrite Hx /=. apply: rt_trans.
+      { apply: rt_steps_app_r. apply: rt_step. by constructor. }
+      apply: rt_step. rewrite /=. by constructor. }
+    apply: rt_trans.
+    { rewrite /=. autorewrite with subst. by apply: eval_rt_steps_subst. }
+    rewrite /=. autorewrite with subst. by apply: rt_refl.
+  - (* JUMP *)
+    move=> i x j v c. rewrite vec_pos_nth vec_change_replace /==> Hx.
+    apply: rt_trans.
+    { apply: rt_steps_app_r.
+      apply: rt_trans.
+      { by apply: eval_rt_steps_subst. }
+      apply: rt_trans.
+      { rewrite /=. autorewrite with subst. do 2 apply: rt_steps_app_r. by apply: eval_rt. }
+      rewrite Hx /=. apply: rt_trans.
+      { apply: rt_steps_app_r. apply: rt_step. by constructor. }
+      apply: rt_step. rewrite /=. by constructor. }
+    apply: rt_trans.
+    { rewrite /=. autorewrite with subst. apply: rt_steps_app_r. by apply: eval_rt_steps_subst. }
+    apply: rt_trans.
+    { rewrite /=. autorewrite with subst. apply: rt_steps_app_r. apply: rt_steps_app_l.
+      apply: eval_rt. by apply: enc_replace_spec. }
+    apply: rt_trans.
+    { apply: rt_steps_app_r. by apply: eval_rt_steps_subst. }
+    apply: rt_trans.
+    { rewrite /=. autorewrite with subst. by apply: eval_rt_steps_subst. }
+    rewrite /=. autorewrite with subst. by apply: rt_refl.
+Qed.
 
 (* \cs.\f.\run.cs *)
 Definition enc_halt := lam (lam (lam (var 2))).
 (* \i.i (halt :: P) *)
 Definition enc_step := lam (apps (var 0) (rev (enc_halt :: map enc_instr (combine (seq 1 (length P)) P)))).
+(* \i.\cs.step i cs recurse *)
+Definition enc_run := lam (lam (apps enc_step [var 1; var 0; enc_recurse])).
 
 Lemma enc_halt_closed : closed enc_halt.
 Proof.
   done.
-Qed.
-
-Lemma eval_enc_halt : eval enc_halt enc_halt.
-Proof.
-  by constructor.
 Qed.
 
 Lemma enc_halt_spec cs : 
@@ -797,10 +846,18 @@ Proof.
   apply: rt_trans.
   { rewrite /=. apply: eval_rt_steps_subst. by constructor. }
   autorewrite with subst. by apply: rt_refl.
+Qed.  
+
+Lemma eval_enc_halt : eval enc_halt enc_halt.
+Proof.
+  by constructor.
 Qed.
 
 #[local] Hint Resolve eval_enc_halt : core.
 #[local] Hint Rewrite enc_halt_closed : subst.
+
+Opaque enc_recurse.
+Opaque enc_halt.
 
 Lemma map_subst_map_enc_instr k t l : map (fun u => subst u k t) (map enc_instr l) = map enc_instr l.
 Proof.
@@ -812,6 +869,34 @@ Proof.
   rewrite /enc_step. move=> k u /=. rewrite subst_apps /=.
   rewrite map_app map_rev map_subst_map_enc_instr /=.
   by autorewrite with subst.
+Qed.
+
+#[local] Hint Rewrite enc_step_closed : subst.
+
+Opaque Nat.sub.
+
+Lemma addr_spec_in_code {l instr r} :
+  P = l ++ instr :: r ->
+  addr (S (length l)) = S (length l).
+Proof.
+  rewrite /addr=> ->. rewrite length_app /=.
+  by have ->: S (length l) - (length l + S (length r)) = 0 by lia.
+Qed.
+
+Lemma addr_spec_out_code {i} : i < 1 \/ S (length P) <= i -> addr i = 0.
+Proof.
+  rewrite /addr => - [?|?].
+  - have ->: i = 0 by lia.
+    by case: (length P).
+  - by have ->: i - length P = S (i - length P - 1) by lia.
+Qed.
+
+Opaque addr.
+
+Lemma map_nth' {X Y : Type} {f : X -> Y} {l i} {d} d' : i < length l -> nth i (map f l) d = f (nth i l d').
+Proof.
+  move=> H. rewrite (nth_indep _ _ (f d')); first by rewrite length_map.
+  by apply: map_nth.
 Qed.
 
 Lemma enc_step_spec l instr r cs :
@@ -866,68 +951,7 @@ Proof.
   by apply: rt_refl.
 Qed.
 
-#[local] Hint Rewrite enc_step_closed : subst.
-Opaque enc_recurse enc_halt enc_step.
-
-Lemma mma_step_sim (instr : MM.mm_instr (Fin.t N)) (p q : mm_state N) :
-  mma_sss instr p q ->
-  clos_refl_trans _ step
-    (apps (enc_instr (fst p, instr)) [enc_regs (snd p); enc_recurse])
-    (apps enc_recurse [pi (addr (fst q)); enc_regs (snd q)]).
-Proof.
-  case.
-  - (* INC *)
-    move=> i x v /=. rewrite vec_change_replace vec_pos_nth.
-    apply: rt_trans.
-    { apply: rt_steps_app_r. by apply: eval_rt_steps_subst. }
-    apply: rt_trans.
-    { apply: rt_steps_app_r. rewrite /=. apply: rt_steps_app_l.
-      autorewrite with subst. apply: eval_rt.
-      apply: enc_replace_spec. apply: nat_succ_spec. by apply: enc_nth_spec. }
-    apply: rt_trans.
-    { apply: rt_steps_app_r. autorewrite with subst. by apply: eval_rt_steps_subst. }
-    apply: rt_trans.
-    { rewrite /=. by apply: eval_rt_steps_subst. }
-    rewrite /=. autorewrite with subst. by apply: rt_refl.
-  - (* DEC *)
-    move=> i x j v. rewrite vec_pos_nth /==> Hx.
-    apply: rt_trans.
-    { apply: rt_steps_app_r.
-      apply: rt_trans.
-      { by apply: eval_rt_steps_subst. }
-      apply: rt_trans.
-      { rewrite /=. autorewrite with subst. do 2 apply: rt_steps_app_r. by apply: eval_rt. }
-      rewrite Hx /=. apply: rt_trans.
-      { apply: rt_steps_app_r. apply: rt_step. by constructor. }
-      apply: rt_step. rewrite /=. by constructor. }
-    apply: rt_trans.
-    { rewrite /=. autorewrite with subst. by apply: eval_rt_steps_subst. }
-    rewrite /=. autorewrite with subst. by apply: rt_refl.
-  - (* JUMP *)
-    move=> i x j v c. rewrite vec_pos_nth vec_change_replace /==> Hx.
-    apply: rt_trans.
-    { apply: rt_steps_app_r.
-      apply: rt_trans.
-      { by apply: eval_rt_steps_subst. }
-      apply: rt_trans.
-      { rewrite /=. autorewrite with subst. do 2 apply: rt_steps_app_r. by apply: eval_rt. }
-      rewrite Hx /=. apply: rt_trans.
-      { apply: rt_steps_app_r. apply: rt_step. by constructor. }
-      apply: rt_step. rewrite /=. by constructor. }
-    apply: rt_trans.
-    { rewrite /=. autorewrite with subst. apply: rt_steps_app_r. by apply: eval_rt_steps_subst. }
-    apply: rt_trans.
-    { rewrite /=. autorewrite with subst. apply: rt_steps_app_r. apply: rt_steps_app_l.
-      apply: eval_rt. by apply: enc_replace_spec. }
-    apply: rt_trans.
-    { apply: rt_steps_app_r. by apply: eval_rt_steps_subst. }
-    apply: rt_trans.
-    { rewrite /=. autorewrite with subst. by apply: eval_rt_steps_subst. }
-    rewrite /=. autorewrite with subst. by apply: rt_refl.
-Qed.
-
-(* \i.\cs.step i cs recurse *)
-Definition enc_run := lam (lam (apps enc_step [var 1; var 0; enc_recurse])).
+Opaque enc_step.
 
 Lemma enc_run_closed : closed enc_run.
 Proof.
@@ -958,6 +982,8 @@ Qed.
 
 Opaque enc_recurse.
 
+#[local] Hint Rewrite subst_apps : subst.
+
 Lemma t_steps_enc_run_enc_step i cs :
   clos_trans term step
     (apps enc_run [pi (addr i); enc_regs cs])
@@ -967,10 +993,11 @@ Proof.
   { apply: t_steps_app_r. apply: t_step. apply: step_app'. by apply: eval_pi. }
   apply: clos_t_rt_t.
   { rewrite /=. apply: t_step. by apply: step_app'. }
-  rewrite /=. autorewrite with subst. by apply: rt_refl.
+  rewrite /=. apply: rt_refl'.
+  by autorewrite with subst.
 Qed.
 
-Opaque enc_instr.
+Opaque enc_step enc_instr.
 
 Lemma enc_run_spec (p q : mm_state N) : @sss_step _ _ (@mma_sss N) (1, P) p q ->
   clos_trans term step
@@ -1003,6 +1030,11 @@ Proof.
   by apply: enc_halt_spec.
 Qed.
 
+Lemma closed_enc_run : closed enc_run.
+Proof.
+  move=> k u. rewrite /enc_run /=. by autorewrite with subst.
+Qed.
+
 Definition sync p t := t = apps enc_run [pi (addr (fst p)); enc_regs (snd p); enc_run].
 
 Lemma sss_step_transport p q s :
@@ -1018,10 +1050,18 @@ Lemma stuck_sss_step_transport p s :
   stuck (sss_step (@mma_sss N) (1, P)) p ->
   sync p s -> terminates step s.
 Proof.
-  move=> /out_code_iff Hp ->.
+  move=> /MMA_computable_to_MMA_mon_computable.out_code_iff Hp ->.
   exists (enc_regs (snd p)). split.
   - by apply: enc_run_spec_out_code.
   - move=> t. intros H. by inversion H.
+Qed.
+
+Lemma sss_step_dec p :
+  (exists q, sss_step (@mma_sss N) (1, P) p q) \/ stuck (sss_step (@mma_sss N) (1, P)) p.
+Proof.
+  have [|] := subcode.in_out_code_dec (fst p) (1, P).
+  - move=> /MMA_computable_to_MMA_mon_computable.in_code_step ?. by left.
+  - move=> /MMA_computable_to_MMA_mon_computable.out_code_iff ?. by right.
 Qed.
 
 Opaque enc_run.
@@ -1038,13 +1078,122 @@ Require Import Undecidability.Synthetic.Definitions.
 (* Halting problem for weak call-by-value lambda-calculus *)
 Definition HaltLclosed (s : {s : term | closed s}) := exists t, eval (proj1_sig s) t.
 
+Lemma MMA_HALTING_terminates_sss_step_iff n (P : list (mm_instr (Fin.t (S n)))) (v : Vector.t nat (S n)) :
+  MMA_HALTING (P, v) <-> terminates (sss_step (@mma_sss (S n)) (1, P)) (1, v).
+Proof.
+  by apply: MMA_computable_to_MMA_mon_computable.sss_terminates_iff.
+Qed.
+
+(*
+Lemma sss_terminates_iff {n s P} : sss_terminates (@mma_sss n) P s <-> terminates (sss_step (@mma_sss n) P) s.
+Proof.
+  split.
+  - move=> [t] [/MMA_computable_to_MMA_mon_computable.sss_compute_iff ? /out_code_iff ?]. by exists t.
+  - move=> [t] [/sss_compute_iff ? /out_code_iff ?]. by exists t.
+Qed.
+*)
+
+Lemma closed_app s t : closed (app s t) -> closed s /\ closed t.
+Proof.
+  move=> H. split=> k u; by move: (H k u)=> [].
+Qed.
+
+Lemma closed_rt_step {s t} :
+  clos_refl_trans term step s t ->
+  closed s ->
+  closed t.
+Proof.
+  elim; by eauto using L_facts.closed_step.
+Qed.
+
+Fixpoint term_size t : nat :=
+  match t with
+  | var _ => 1
+  | app s t => 1 + term_size s + term_size t
+  | lam s => 1 + term_size s
+  end.
+
+Lemma not_closed_var n : closed (var n) -> False.
+Proof.
+  move=> /(_ n (var (S n))) /=.
+  rewrite Nat.eqb_refl=> - []. lia.
+Qed.
+
+Lemma closed_not_lambda_step s :
+  closed s ->
+  (not (L_facts.lambda s)) ->
+  exists t, step s t.
+Proof.
+  elim /(Nat.measure_induction _ term_size) : s.
+  move=> [n|{}s t|?].
+  - by move=> ? /not_closed_var.
+  - move=> IH /closed_app [].
+    move: s t IH=> [?|??|?].
+    + by move=> ?? /not_closed_var.
+    + move=> t /[apply] IH _ _.
+      case: IH.
+      * rewrite /=. lia.
+      * by case.
+      * move=> *. eexists. apply: L_facts.stepAppL. by eassumption.
+    + move=> [?|??|?].
+      * by move=> ?? /not_closed_var.
+      * move=> IH ? /IH {}IH _.
+        case: IH.
+        ** rewrite /=. lia.
+        ** by case.
+        ** move=> *. eexists. apply: L_facts.stepAppR. by eassumption.
+      * move=> *. eexists. by constructor.
+  - move=> _ _ H. exfalso. apply: H. by eexists.
+Qed.
+
+Lemma closed_stuck_lambda t :
+  closed t ->
+  stuck step t ->
+  L_facts.lambda t.
+Proof.
+  move=> /closed_not_lambda_step.
+  move: t=> [?|??|?].
+  - case.
+    + by case.
+    + by move=> t ? /(_ t).
+  - case.
+    + by case.
+    + by move=> t ? /(_ t).
+  - move=> *. by eexists.
+Qed.
+
+Lemma steps_stuck_eval s t :
+  closed s ->
+  clos_refl_trans term step s t ->
+  stuck step t ->
+  eval s t.
+Proof.
+  move=> Hs Hst Ht. apply /L_facts.eval_iff. split.
+  - by apply /star_rt_steps_iff.
+  - apply: closed_stuck_lambda; last done.
+    by apply: (closed_rt_step Hst).
+Qed.
+
+Lemma stuck_lam s : stuck step (lam s).
+Proof.
+  move=> t H. by inversion H.
+Qed.
+
+Lemma eval_steps_stuck s t : eval s t -> terminates L_facts.step s.
+Proof.
+  move=> /L_facts.eval_iff [?] [?] ?. subst.
+  eexists. split.
+  - apply /star_rt_steps_iff. by eassumption.
+  - by apply: stuck_lam.
+Qed.
+
 Lemma reduction n : @MMA_HALTING (S n) ⪯ HaltLclosed.
 Proof.
   unshelve eexists.
   - intros [P v]. exists (apps (enc_run P) [pi P (addr P 1); enc_regs v; enc_run P]).
     apply closed_apps_enc_run.
   - intros [P v]. split.
-    + intros ?%sss_terminates_iff.
+    + intros ?%MMA_HALTING_terminates_sss_step_iff.
       destruct (@terminates_transport _ _
         (sss_step (@mma_sss (S n)) (1, P))
         L_facts.step
@@ -1058,14 +1207,14 @@ Proof.
       exists t. cbn. eapply steps_stuck_eval; [|assumption..].
       apply closed_apps_enc_run.
     + intros [t Ht%eval_steps_stuck]. cbn in Ht.
-      apply sss_terminates_iff.
+      apply MMA_HALTING_terminates_sss_step_iff.
       apply (@terminates_reflection _ _ 
         (sss_step (@mma_sss (S n)) (1, P))
         L_facts.step
         (sync P)
         L_facts.uniform_confluence
         (@sss_step_transport _ P)
-        (fun p => sss_step_or_stuck p 1 P)
+        (@sss_step_dec _ P)
         (1, v)
         _
         eq_refl
@@ -1080,7 +1229,70 @@ Fixpoint fin_seq n : list (Fin.t n) :=
   | S n => Fin.F1 :: map Fin.FS (fin_seq n)
   end.
 
+Lemma rt_steps_apps_r s ts t :
+  clos_refl_trans _ step s t -> clos_refl_trans _ step (apps s ts) (apps t ts).
+Proof.
+  elim: ts s t; first done.
+  move=> ?? IH ??? /=. apply: IH.
+  by apply: rt_steps_app_r.
+Qed.
+
 Opaque Vector.to_list Fin.L.
+
+Lemma combine_map_l {A B C} (f : A -> B) (l : list A) (r : list C) :
+  combine (map f l) r = map (fun '(x, y) => (f x, y)) (combine l r).
+Proof.
+  elim: l r; first done.
+  move=> > IH [|? r]; first done.
+  move=> /=. by rewrite IH.
+Qed.
+
+(*
+Fixpoint fin_add n : forall m, Fin.t m -> Fin.t (n + m) :=
+  match n with
+  | 0 => fun m x => x
+  | S n => fun m x => Fin.FS (fin_add n m x)
+  end.
+
+Definition enc_set_state l k n : term :=
+  apps (enc_regs (Vector.const 0 ((S l) + k + n)))
+  (map (fun '(x, i) => app (enc_replace (Fin.L n (fin_add (S l) _ x))) (var i)) (combine (fin_seq k) (rev (seq 0 k)))).
+
+Opaque enc_replace.
+
+Lemma substs_enc_set_state_aux l k n (v : Vector.t nat k) :
+  clos_refl_trans _ step
+    (substs 0 (rev (map nat_enc (VectorDef.to_list v))) (enc_set_state l k n))
+    (enc_regs (fold_left (fun w '(c, x) => Vector.replace w (Fin.L n (fin_add (S l) _ x)) c) (combine (Vector.to_list v) (fin_seq k)) (Vector.const 0 ((S l) + k + n)))).
+Proof.
+  rewrite /enc_set_state.
+  move: (Vector.const 0 ((S l) + k + n))=> cs.
+  rewrite substs_apps substs_closed; first by apply: enc_regs_closed.
+  elim: v l cs.
+  - move=> l cs /=. by apply: rt_refl.
+  - move=> c {}k v IH l cs.
+    have ->: rev (seq 0 (S k)) = k :: rev (seq 0 k).
+    { have ->: S k = k + 1 by lia.
+      by rewrite seq_app rev_app_distr. }
+    apply: rt_trans.
+    { rewrite /=. apply: rt_steps_apps_r. rewrite substs_closed; first by apply: enc_replace_closed.
+      apply: eval_rt. apply: enc_replace_spec.
+      rewrite -Vector.to_list_map -Vector.to_list_rev -Vector.to_list_nth_order.
+      rewrite -Vector.map_rev nth_order_map. by apply: eval_nat_enc. }
+    rewrite combine_map_l (map_map (fun '(x, y) => (Fin.FS x, y))).
+    apply: rt_trans.
+    { set cs' := (cs' in enc_regs cs').
+      rewrite Vector.to_list_cons /=.
+      have := IH (S l) cs'.
+     apply: IH. }
+      
+       Search (VectorDef.nth_order).
+
+       apply: nat_enc_spec. }
+     rewrite map_cons.
+     by done.
+
+*)
 
 (* apps (enc_regs (Vector.const 0 (1 + k + n))) (Vector.to_list (Vector.map (fun x => enc_replace (Fin.L n (Fin.FS x))) (rev_vec_seq k)))*)
 Definition enc_set_state k n : term :=
@@ -1129,6 +1341,14 @@ Proof.
 Qed.
 
 Print Assumptions substs_enc_set_state_aux.
+
+Lemma vec_eq_nth {A : Type} (n : nat) (v1 v2 : VectorDef.t A n) :
+  (forall p : Fin.t n, Vector.nth v1 p = Vector.nth v2 p) <-> v1 = v2.
+Proof.
+  split.
+  - move=> ?. apply /Vector.eq_nth_iff. by move=> i ? <-.
+  - move=> /Vector.eq_nth_iff H *. by apply: H.
+Qed.
 
 Lemma substs_enc_set_state k n v :
   clos_refl_trans _ step
@@ -1196,7 +1416,7 @@ Qed.
 
 Opaque enc_run pi enc_set_state enc_nth.
 
-Lemma enc_init_spec {k n} (P : list (MM.mm_instr (Fin.t (1 + k + n)))) (v : Vector.t nat k) :
+Lemma enc_init_spec {k n} (P : list (mm_instr (Fin.t (1 + k + n)))) (v : Vector.t nat k) :
   clos_refl_trans _ step
     (Vector.fold_left (fun (s : term) c => app s (nat_enc c))
       (lams k (apps (enc_run P) [pi P (addr P 1); enc_set_state k n; enc_run P; enc_nth (@Fin.F1 (k + n))])) v)
@@ -1219,6 +1439,34 @@ Proof.
   by apply: rt_refl.
 Qed.
 
+(* TODO use comb_proc_red *)
+
+Lemma eval_rt_steps_eval s t u : eval s t -> clos_refl_trans _ step s u -> eval u t.
+Proof.
+  move=> /L_facts.eval_iff [+] [s'] ?. subst.
+  move=> + /star_rt_steps_iff.
+  move=> /L_facts.confluence /[apply] - [?] [H1 H2].
+  apply /L_facts.eval_iff.
+  have Hs' : L_facts.lambda (lam s') by eexists.
+  split.
+  - have := L_facts.lam_terminal Hs'.
+    move: H1 H2 => []; first done.
+    by move=> > + _ _ H => /H.
+  - by eexists.
+Qed.
+
+Lemma clos_trans_flip {X : Type} {R : X -> X -> Prop} {x y} : clos_trans _ R x y ->
+  clos_trans _ (fun y x => R x y) y x.
+Proof. by elim; eauto using clos_trans. Qed.
+
+Lemma nat_enc_inj n m : nat_enc n = nat_enc m -> n = m.
+Proof.
+  elim: n m.
+  - by case.
+  - move=> n IH [|m] /=; first done.
+    by move=> [/IH] <-.
+Qed.
+
 Theorem MMA_computable_to_L_computable_closed {k} (R : Vector.t nat k -> nat -> Prop) :
   MMA_computable R -> L_computable_closed R.
 Proof.
@@ -1229,14 +1477,14 @@ Proof.
   split.
   - intros u ?.
     rewrite subst_lams subst_apps !map_cons subst_enc_set_state.
-    by rewrite !enc_run_closed pi_addr_closed enc_nth_closed.
+    by rewrite !closed_enc_run pi_addr_closed enc_nth_closed.
   - move=> v. split.
     + move=> m. rewrite HP. split.
       * intros [c [v' [H1 H2]]].
         apply /L_facts.eval_iff. split; last by (case: (m); eexists).
         apply /star_rt_steps_iff. apply: rt_trans.
         { by apply: enc_init_spec. }
-        move=> /sss_compute_iff in H1.
+        move=> /MMA_computable_to_MMA_mon_computable.sss_compute_iff in H1.
         have := @clos_refl_trans_transport _ _
         (sss_step (@mma_sss ((1 + k + n))) (1, P))
         L_facts.step
@@ -1261,17 +1509,17 @@ Proof.
         move E: (apps _ _) => t H.
         elim: H i v E {H' Hi}.
         move=> {}t IH1 IH2 i v ?. subst t.
-        have [[[j w]]|] := sss_step_or_stuck (i, v) 1 P.
+        have [[[j w]]|] := @sss_step_dec (k + n) P (i, v).
         ** move=> /[dup] Hvw /enc_run_spec /=.
            move=> /(@t_steps_app_r _ _ (enc_nth (@Fin.F1 (k + n)))).
            move=> /[dup] /(@clos_trans_clos_refl_trans term) /eval_rt_steps_eval H' + /H'.
            move=> /clos_trans_flip /IH2 /(_ _ _ eq_refl) /[apply].
            move=> [c] [v'] [??]. exists c, v'. split; last done.
            apply: sss_compute_trans; last by eassumption.
-           apply /sss_compute_iff.
+           apply /MMA_computable_to_MMA_mon_computable.sss_compute_iff.
            by apply: rt_step.
-        ** move=> /[dup] /out_code_iff /enc_run_spec_out_code H.
-           move=> /[dup] /out_code_iff H''.
+        ** move=> /[dup] /MMA_computable_to_MMA_mon_computable.out_code_iff /enc_run_spec_out_code H.
+           move=> /[dup] /MMA_computable_to_MMA_mon_computable.out_code_iff H''.
            move=> /stuck_sss_step_transport => /(_ _ eq_refl) [t] H'.
            move: H=> /(rt_steps_app_r _ _ (enc_nth (@Fin.F1 (k + n)))).
            move=> /eval_rt_steps_eval /[apply].
@@ -1282,9 +1530,10 @@ Proof.
            move=> /nat_enc_inj <-.
            exists i, (snd (@Vector.splitat _ 1 (k + n) v)).
            split; last done.
-           apply /sss_compute_iff.
-           rewrite (Vector.eta v).
-           by apply: rt_refl.
+           apply /MMA_computable_to_MMA_mon_computable.sss_compute_iff.
+           apply: rt_refl'. congr pair.
+           rewrite [LHS](@MMA_computable_to_MMA_mon_computable.Facts.vec_append_splitat _ 1 (k + n)).
+           by rewrite (Vector.eta v).
     + move=> o /eval_rt_steps_eval => /(_ _ (enc_init_spec _ _)).
       move: (Vector.append _ _)=> {}v /[dup] /eval_steps_stuck H'.
       have /(@Acc_clos_trans term) := @terminating_Acc _ _ L_facts.uniform_confluence _ H'.
@@ -1292,12 +1541,12 @@ Proof.
       move E: (apps _ _) => t H.
       elim: H i v E {H'}.
       move=> {}t IH1 IH2 i v ?. subst t.
-      have [[[j w]]|] := sss_step_or_stuck (i, v) 1 P.
+      have [[[j w]]|] := @sss_step_dec (k + n) P (i, v).
       * move=> /enc_run_spec /=.
         move=> /(@t_steps_app_r _ _ (enc_nth (@Fin.F1 (k + n)))).
         move=> /[dup] /(@clos_trans_clos_refl_trans term) /eval_rt_steps_eval H' + /H'.
         by move=> /clos_trans_flip /IH2 /(_ _ _ eq_refl) /[apply].
-      * move=> /[dup] /out_code_iff /enc_run_spec_out_code H.
+      * move=> /[dup] /MMA_computable_to_MMA_mon_computable.out_code_iff /enc_run_spec_out_code H.
         move=> /stuck_sss_step_transport => /(_ _ eq_refl) [t] H'.
         move: H=> /(rt_steps_app_r _ _ (enc_nth (@Fin.F1 (k + n)))).
         move=> /eval_rt_steps_eval /[apply].
